coq/theories/automation/Automation.v
@@ -1,20 +1,27 @@
+From impboot Require Import utils.Core.
 Require Import impboot.functional.FunValues.
 Require Import impboot.functional.FunSyntax.
 Require Import impboot.functional.FunSemantics.
 Require Import impboot.automation.AutomationLemmas.
 Require Import impboot.utils.Llist.
-Require Import Coq.Bool.Bool.
-Require Import Coq.Lists.List.
-Import ListNotations.
-Require Import Lia Nat Arith.
+
+Ltac rewrite_let := match goal with
+| [ |- context C [?subterm] ] =>
+  match subterm with
+  | let x := ?a in @?b x =>
+    let C' := context C [b a] in
+    change C'
+  end
+end.
 
 Definition empty_state : state := init_state lnil [].
 
 (* TODO(kπ) figure out a good example, this one gets constant folded *)
-Example arith_example : forall n m,
-  exists prog, Env.empty |- (prog, empty_state) ---> ([Num ((fun x => x + n - m) 1)], empty_state).
+(* Example arith_example : forall n m,
+  exists prog, Env.empty |- (prog, empty_state) ---> ([Num (let x := 1 in x + n - m)], empty_state).
 Proof.
   intros.
+  rewrite_let.
   eexists. (* TODO(kπ) this simplifies my function :/ Is this a problem with normal code?*)
   eapply auto_let; eauto; intros.
   repeat match goal with
@@ -22,7 +29,7 @@ Proof.
   | |- context[_ - _] => eapply auto_num_sub; eauto
   end.
   (* TODO(kπ) *)
-Qed.
+Qed. *)
 
 (*
 TODO(kπ) Problems:
