coq/theories/utils/Core.v
@@ -1,0 +1,59 @@
+From Coq Require Export
+  Lists.List
+  Bool.Bool
+  Strings.Ascii
+  Strings.String
+  Numbers.DecimalString
+  Arith.PeanoNat.
+Export ListNotations.
+Require Export
+  Lia
+  String
+  Nat
+  Arith
+  ZArith.
+From coqutil Require Import dlet.
+
+(* d/let *)
+
+Notation "'letd' x := e1 'in' e2" :=
+  (dlet e1 (fun x => e2))
+  (at level 200).
+
+Notation
+  "'letd' ''(' x , y ')' := val 'in' body" :=
+(dlet val
+    (fun v =>
+       let x := fst v in
+       let y := snd v in
+       body))
+(at level 200, only parsing).
+
+Notation
+  "'letd' ''(' x , y , z ')' := val 'in' body" :=
+(dlet val
+    (fun v =>
+       let x := fst (fst v) in
+       let y := snd (fst v) in
+       let z := snd v in
+       body))
+(at level 200, only parsing).
+
+(* CASE *)
+
+Definition list_CASE {A B} (l : list A) (fnil : B) (fcons : A -> list A -> B) : B :=
+  match l with
+  | [] => fnil
+  | x :: xs => fcons x xs
+  end.
+
+Definition option_CASE {A B} (o : option A) (fnone : B) (fsome : A -> B) : B :=
+  match o with
+  | None => fnone
+  | Some x => fsome x
+  end.
+
+Definition pair_CASE {A1 A2 B} (p : A1 * A2) (f: A1 -> A2 -> B) : B :=
+  match p with
+  | (x, y) => f x y
+  end.
